\clearpage

\subsection{Translucent with 1+1 Protection}\label{ILP_Transluc_Protection}
\begin{tcolorbox}	
\begin{tabular}{p{2.75cm} p{0.2cm} p{10.5cm}} 	
\textbf{Student Name}  &:& Tiago Esteves    (October 03, 2017 - )\\
\textbf{Goal}          &:& Implement the ILP model for the translucent transport mode with 1 plus 1 protection.
\end{tabular}
\end{tcolorbox}
\vspace{11pt}

Here, in this case, we must take into account table \ref{description_transluc}, previously mentioned, in order to better understand the objective function.\\

The objective function of following the ILP is a minimization of the sum of two equations: the cost of the links \ref{Capex_Link} and cost of the nodes \ref{Capex_Node} where in this case we have in consideration the electric cost and the optical cost.
In this case the value of $P_{exc,c,n}$ is obtained by equation \ref{EXC_pexc_translucent} and the value of $P_{oxc,n}$ is obtained by equation \ref{OXC_poxc_translucent}.\\

\vspace{17pt}
The objective function, to be minimized, is the expression \ref{ILPOpaque_CAPEX}.\\

$subject$ $to$
\begin{equation}
\sum_{j\textbackslash \{o\}} Ls_{ij}^{od} = D_{odc}  \qquad \qquad \qquad \qquad \qquad \qquad \qquad \qquad \qquad
\forall(o,d) : o < d, \forall i: i = o
\label{ILPTranslucp1}
\end{equation}

\begin{equation}
\sum_{j\textbackslash \{i,o\}} Ls_{ij}^{od} = \sum_{j\textbackslash \{i,d\}} Ls_{ji}^{od} \qquad \qquad \qquad \qquad \qquad \qquad \qquad
\forall(o,d) : o < d, \forall i: i \neq o,d
\label{ILPTranslucp2}
\end{equation}

\begin{equation}
\sum_{j\textbackslash \{d\}} Ls_{ji}^{od} = D_{odc} \qquad \qquad \qquad \qquad \qquad \qquad \qquad \qquad \qquad
\forall(o,d) : o < d, \forall i: i = d
\label{ILPTranslucp3}
\end{equation}

\begin{equation}
\sum_{(o,d):o<d} B(c) Ls_{ij}^{od} \leq  100 \lambda_{od} \qquad \qquad \qquad \qquad \qquad \qquad \qquad \qquad \qquad \qquad \qquad
\forall (i,j)
\label{ILPTranslucp4}
\end{equation}

\begin{equation}
\sum_{j\textbackslash \{o\}} f_{ij}^{od} = \lambda_{od}  \qquad \qquad \qquad \qquad \qquad \qquad \qquad \qquad \qquad
\forall(o,d) : o < d, \forall i: i = o
\label{ILPTranslucp6}
\end{equation}

\begin{equation}
\sum_{j\textbackslash \{o\}} f_{ij}^{od} = \sum_{j\textbackslash \{d\}} f_{ji}^{od} \qquad \qquad \qquad \qquad \qquad \qquad \qquad \qquad
\forall(o,d) : o < d, \forall i: i \neq o,d
\label{ILPTranslucp7}
\end{equation}

\begin{equation}
\sum_{j\textbackslash \{d\}} f_{ji}^{od} = \lambda_{od}  \qquad \qquad \qquad \qquad \qquad \qquad \qquad \qquad \qquad
\forall(o,d) : o < d, \forall i: i = d
\label{ILPTranslucp8}
\end{equation}

\begin{equation}
\sum_{j\textbackslash \{o\}} fp_{ij}^{od} = \lambda_{od}  \qquad \qquad \qquad \qquad \qquad \qquad \qquad \qquad \qquad
\forall(o,d) : o < d, \forall i: i = o
\label{ILPTranslucp6a}
\end{equation}

\begin{equation}
\sum_{j\textbackslash \{o\}} fp_{ij}^{od} = \sum_{j\textbackslash \{d\}} f_{ji}^{od} \qquad \qquad \qquad \qquad \qquad \qquad \qquad \qquad
\forall(o,d) : o < d, \forall i: i \neq o,d
\label{ILPTranslucp7a}
\end{equation}

\begin{equation}
\sum_{j\textbackslash \{d\}} fp_{ji}^{od} = \lambda_{od}  \qquad \qquad \qquad \qquad \qquad \qquad \qquad \qquad \qquad
\forall(o,d) : o < d, \forall i: i = d
\label{ILPTranslucp8a}
\end{equation}

\begin{equation}
\sum_{(o,d):o<d} \left(f_{ij}^{od}  + fp_{ij}^{od}\right) \leq \lambda_{od}  \qquad \qquad \qquad \qquad \qquad \qquad \qquad \qquad \qquad
\forall (o,d), (i,j)
\label{ILPTranslucpx}
\end{equation}

\begin{equation}
\sum_{(o,d):o<d} \left( f_{ij}^{od} + f_{ji}^{od} + fp_{ij}^{od} + fp_{ji}^{od} \right) \leq K_{ij} G_{ij}
\qquad \qquad \qquad \qquad \qquad
\forall (i,j) : i < j
\label{ILPTranslucp9}
\end{equation}

\begin{equation}
L_{ij}^{od} \geq 0;
\qquad \qquad \qquad \qquad \qquad \qquad \qquad \qquad \qquad \qquad \qquad \qquad
\forall (i,j) , \forall (o,d) : o < d
\label{ILPTranslucp5}
\end{equation}

\begin{equation}
f_{ij}^{od}, fp_{ij}^{od} \geq 0
\qquad \qquad \qquad \qquad \qquad \qquad \qquad \qquad \qquad \qquad \qquad \qquad
\forall (i,j) \forall (o,d)
\label{ILPTranslucp10}
\end{equation}	

